erasure/theories/ETyping.v
@@ -16,15 +16,15 @@ Set Asymmetric Patterns.
  *)
 (** ** Environment lookup *)
 
-Fixpoint lookup_env (Σ : global_declarations) (id : ident) : option global_decl :=
+Fixpoint lookup_env (Σ : global_declarations) id : option global_decl :=
   match Σ with
   | nil => None
   | hd :: tl =>
-    if ident_eq id hd.1 then Some hd.2
+    if kername_eq_dec id hd.1 then Some hd.2
     else lookup_env tl id
   end.
 
-Definition declared_constant (Σ : global_declarations) (id : ident) decl : Prop :=
+Definition declared_constant (Σ : global_declarations) id decl : Prop :=
   lookup_env Σ id = Some (ConstantDecl decl).
 
 Definition declared_minductive Σ mind decl :=
