pcuic/theories/PCUICAstUtils.v
@@ -30,7 +30,7 @@ Fixpoint string_of_term (t : term) :=
   | tLetIn na b t' t => "LetIn(" ++ string_of_name na ++ "," ++ string_of_term b
                                  ++ "," ++ string_of_term t' ++ "," ++ string_of_term t ++ ")"
   | tApp f l => "App(" ++ string_of_term f ++ "," ++ string_of_term l ++ ")"
-  | tConst c u => "Const(" ++ c ++ "," ++ string_of_universe_instance u ++ ")"
+  | tConst c u => "Const(" ++ string_of_kername c ++ "," ++ string_of_universe_instance u ++ ")"
   | tInd i u => "Ind(" ++ string_of_inductive i ++ "," ++ string_of_universe_instance u ++ ")"
   | tConstruct i n u => "Construct(" ++ string_of_inductive i ++ "," ++ string_of_nat n ++ ","
                                     ++ string_of_universe_instance u ++ ")"
@@ -116,7 +116,7 @@ Proof.
     apply (List.firstn decl.(ind_npars)) in names.
     apply (List.firstn decl.(ind_npars)) in types.
     refine (List.combine _ _).
-    exact (List.map get_ident names).
+    exact (List.map string_of_name names).
     exact (List.map LocalAssum types).
   - refine (List.map _ decl.(ind_bodies)).
     intros [].
