pcuic/theories/PCUICLiftSubst.v
@@ -1648,7 +1648,7 @@ Lemma term_forall_ctx_list_ind :
     (forall Γ (n : name) (t : term),
         P Γ t -> forall t0 : term, P Γ t0 -> forall t1 : term, P (vdef n t t0 :: Γ) t1 -> P Γ (tLetIn n t t0 t1)) ->
     (forall Γ (t u : term), P Γ t -> P Γ u -> P Γ (tApp t u)) ->
-    (forall Γ (s : String.string) (u : list Level.t), P Γ (tConst s u)) ->
+    (forall Γ s (u : list Level.t), P Γ (tConst s u)) ->
     (forall Γ (i : inductive) (u : list Level.t), P Γ (tInd i u)) ->
     (forall Γ (i : inductive) (n : nat) (u : list Level.t), P Γ (tConstruct i n u)) ->
     (forall Γ (p : inductive * nat) (t : term),
