test-suite/proj.v
@@ -1,4 +1,4 @@
-Require Import MetaCoq.Template.Loader.
+Require Import MetaCoq.Template.All.
 Require Import String.
 Set Primitive Projections.
 
@@ -23,7 +23,38 @@ Proof.
    |- ?T => quote_term T (fun x => pose (qgoal:=x))
   end.
   match goal with
-    H:= context [Ast.tProj (BasicAst.mkInd "MetaCoq.TestSuite.proj.Eq"%string 0, 1, 0) _] |- _ => idtac
+    H:= context [Ast.tProj (BasicAst.mkInd _ 0, 1, 0) _] |- _ => idtac
   end.
   reflexivity.
 Qed.
+
+Record prod' A B : Type :=
+  pair' { fst' : A ; snd' : B }.
+Arguments fst' {A B} _.
+Arguments snd' {A B} _.
+
+MetaCoq Test Quote ((pair' _ _ true 4).(snd')).
+
+MetaCoq Test Quote prod'.
+
+Require Import List String.
+Import ListNotations.
+
+
+Definition qprod' := mkInd (MPfile ["proj"; "TestSuite"; "MetaCoq"], "prod'") 0.
+Definition qnat := mkInd (MPfile ["Datatypes"; "Init"; "Coq"], "nat") 0.
+Definition qbool := mkInd (MPfile ["Datatypes"; "Init"; "Coq"], "bool") 0.
+
+MetaCoq Unquote Definition x := (tProj (qprod', 2, 1)
+   (tApp (tConstruct qprod' 0 nil)
+      [tInd qbool nil;
+      tInd qnat nil;
+      tConstruct qbool 0 nil;
+      tApp (tConstruct qnat 1 nil)
+        [tApp (tConstruct qnat 1 nil)
+           [tApp (tConstruct qnat 1 nil)
+              [tApp (tConstruct qnat 1 nil)
+                 [tConstruct qnat 0 nil]]]]])).
+
+Check (eq_refl : x = snd' {| fst' := true; snd' := 4 |}).
+Check (eq_refl : x = 4).
